relecture1

theories/SLFHprop.v
@@ -39,15 +39,15 @@ Local Coercion string_to_var (x:string) : var := x.
 (** ** Syntax and semantics *)
 
 (** We here assume an imperative programming language with a formal semantics.
-    Such a language is described in file [Semantics.v], but we do not need to
+    Such a language is described in file [SLFDirect.v], but we do not need to
     know about the details for now. All we need to know is that there exists:
 
     - a type of terms, written [trm],
     - a type of values, written [val],
-    - a type of states, written [heap],
+    - a type of states, written [state],
     - a big-step evaluation judgment, written [eval h1 t h2 v], asserting that,
       starting from state [s1], the evaluation of the term [t] terminates in
-      the state [s2] and produces the value [v]. 
+      the state [s2] and produces the value [v].
 
 [[
     Check eval : state -> trm -> state -> val -> Prop.
@@ -56,10 +56,9 @@ Local Coercion string_to_var (x:string) : var := x.
 
 (** At this point, we don't need to know the exact grammar of terms and values.
     Let's just give one example to make things concrete. Consider the function:
-      [fun x => if x then 0 else 1]. 
+      [fun x => if x then 0 else 1].
 
-    In the language described in the file [Semantics.v], it can be
-    written in raw syntax as: *)
+    In the language that we consider, it can be written in raw syntax as: *)
 
 Definition example_trm : trm :=
   trm_fun "x" (trm_if (trm_var "x") (trm_val (val_int 0)) (trm_val (val_int 1))).
@@ -76,7 +75,7 @@ Definition example_trm' : trm :=
 (** ** Description of the state *)
 
 (** By convention, we use the type [state] describes a full state of memory,
-    and introduce the type [heap] to describe just a piece of state. *) 
+    and introduce the type [heap] to describe just a piece of state. *)
 
 Definition heap := state.
 
@@ -89,7 +88,11 @@ Definition heap := state.
     A state is a finite map from locations to values.
       [Definition state := fmap loc val.] *)
 
-(** The main operations and predicates on the state are as follows.
+(** The main operations and predicates on the state are as follows:
+    empty state, singleton state, union of two states (union is
+    symmetric only if the two arguments have disjoint domains),
+    and definition of disjointness.
+
 [[
     Check Fmap.empty : heap.
 
@@ -107,12 +110,11 @@ Definition heap := state.
 
 (** In Separation Logic (SL), the state is described using "heap predicates",
     which are predicate over pieces of state.
-    We let [hprop] denote the type of heap predicates. *)
+    Let [hprop] denote the type of heap predicates. *)
 
 Definition hprop := heap -> Prop.
 
-(** Thereafter, we use the words "heap" and "state" interchangeably,
-    and let [H] range over heap predicates. *)
+(** Thereafter, let [H] range over heap predicates. *)
 
 Implicit Type H : hprop.
 
@@ -169,7 +171,7 @@ Notation "H1 '\*' H2" := (hstar H1 H2) (at level 41, right associativity).
     The generalized notation [\exists x1 ... xn, H] is also available.
 
     The definition of [hexists] is a bit technical. It may be skipped 
-    in first reading. additional explanations are given further on. *)
+    in first reading. Additional explanations are provided further on. *)
 
 Definition hexists A (J:A->hprop) : hprop :=
   fun (h:heap) => exists x, J x h.
@@ -180,8 +182,8 @@ Notation "'\exists' x1 .. xn , H" :=
    format "'[' '\exists' '/ '  x1  ..  xn , '/ '  H ']'").
 
 (** The "top" heap predicate, written [\Top], holds of any heap predicate.
-    It plays a useful role for denoting pieces of state that needs to be discarded,
-    to reflect in the logic the action of the garbage collector. *)
+    It plays a useful role for denoting pieces of state that needs to be
+    discarded, reflecting in the logic the action of the garbage collector. *)
 
 Definition htop : hprop :=
   fun (h:heap) => True.
@@ -193,9 +195,9 @@ Notation "\Top" := (htop).
 (** ** Extensionality for heap predicates *)
 
 (** To work in Separation Logic, it is extremely convenient
-    (if not absolutely necessary) to be able to state equalities
-    between heap predicates. For example, in the next chapter
-    we will establish associativity for the star operator: *)
+    to be able to state equalities between heap predicates. 
+    For example, in the next chapter, we will establish associativity
+    for the star operator, a property stated as an equality: *)
 
 Parameter hstar_assoc : forall H1 H2 H3,
   (H1 \* H2) \* H3 = H1 \* (H2 \* H3).
@@ -230,7 +232,7 @@ Proof using. applys predicate_extensionality. Qed.
 
 (** A postcondition characterizes both an output value and an output state.
     In SL, a postcondition is thus a relation of type [val -> state -> Prop],
-    which is equivalent to [val -> hprop]. 
+    which is equivalent to [val -> hprop].
 
     Thereafter, we let [Q] range over postconditions. *)
 
@@ -266,7 +268,7 @@ Proof using. applys functional_extensionality. Qed.
     the definition of a Separation Logic triple, let us first give
     the definition of a Hoare triple and state the much-desired frame rule. *)
 
-(** A Hoare triple, written [{H}t{Q}] on paper, and here written
+(** A Hoare triple, written [{H} t {Q}] on paper, and here written
     [hoare t H Q], asserts that starting from a state [s] satisfying
     the precondition [H], the term [t] evaluates to a value [v] and to
     a state [s'] that, together, satisfy the postcondition [Q]. Formally: *)
@@ -281,25 +283,26 @@ Definition hoare (t:trm) (H:hprop) (Q:val->hprop) : Prop :=
 (** The frame rule asserts that if one can derive a specification of
     the form [triple H t Q] for a term [t], then one should be able
     to automatically derive [triple (H \* H') t (Q \*+ H')] for any [H'].
+
     Intuitively, if [t] executes safely in a heap [H], it should behave
     similarly in any extension of [H] with a disjoint part [H'], moreover
     its evaluation should leave this piece of state [H'] unmodified until
-    the end. 
+    the end.
 
     The following definition of a Separation Logic triple builds upon
     that of a Hoare triple by "baking in" the frame rule. *)
 
-Definition SL_triple (t:trm) (H:hprop) (Q:val->hprop) : Prop :=
+Definition triple1 (t:trm) (H:hprop) (Q:val->hprop) : Prop :=
   forall (H':hprop), hoare t (H \* H') (Q \*+ H').
 
 (** This definition inherently satisfies the frame rule, as we show
     below, by exploiting the associativity of the star operator. *)
 
-Lemma SL_triple_frame : forall t H Q H', 
-  SL_triple t H Q ->
-  SL_triple t (H \* H') (Q \*+ H').
+Lemma triple1_frame : forall t H Q H', 
+  triple1 t H Q ->
+  triple1 t (H \* H') (Q \*+ H').
 Proof using.
-  introv M. unfold SL_triple in *. rename H' into H1. intros H2.
+  introv M. unfold triple1 in *. rename H' into H1. intros H2.
   specializes M (H1 \* H2).
   (* [M] matches the goal up to rewriting for associativity. *)
   applys_eq M 1 2.
@@ -307,7 +310,7 @@ Proof using.
   { applys qprop_eq. intros v. rewrite hstar_assoc. auto. }
 Qed.
 
-(** The definition of [SL_triple] presented above can be used as such for
+(** The definition of [triple] presented above can be used as such for
     dealing with languages that feature explicit deallocation. However,
     for a programming language equipped with a garbage collector, we need
     one additional tweak, to account for the fact that a postcondition may
@@ -323,11 +326,11 @@ Qed.
     become useless. Concretely, we need the rule shown below to hold.
     The [\Top] predicate captures any (un)desired piece of state. *)
 
-Parameter SL_triple_htop_post : forall t H Q,
-  SL_triple t H (Q \*+ \Top) ->
-  SL_triple t H Q.
+Parameter triple_htop_post : forall t H Q,
+  triple t H (Q \*+ \Top) ->
+  triple t H Q.
 
-(** The rule above is not satisfied by the definition of [SL_triple].
+(** The rule above is not satisfied by the definition of [triple].
     However, it can be satisfied by applying just a minor tweak
     to the definition. Concretely, we augment the postcondition of
     the underlying Hoare triple with an extra [\Top], which is able
@@ -343,7 +346,7 @@ Definition triple (t:trm) (H:hprop) (Q:val->hprop) : Prop :=
     pieces of postconditions holds, and that the frame rule still
     holds. The proof of these two results is studied further. *)
 
-Parameter triple_htop_post : forall t H Q,
+Parameter triple_htop_post' : forall t H Q,
   triple t H (Q \*+ \Top) ->
   triple t H Q.
 
@@ -373,7 +376,10 @@ Notation "h1 \u h2" := (Fmap.union h1 h2) (at level 37, right associativity).
 (** ** Introduction and inversion lemmas for basic operators *)
 
 (** The following lemmas help getting a better understanding
-    of the meaning of the Separation Logic combinators. *)
+    of the meaning of the Separation Logic combinators.
+
+    For each operator, there is one introduction lemma and one
+    inversion lemma. *)
 
 Implicit Types P : Prop.
 
@@ -530,14 +536,14 @@ Lemma incr_applied : forall (p:loc) (n:int),
 Proof using. reflexivity. Qed.
 
 (** A specification lemma for [incr] takes the form [triple (incr p) H Q].
-    The precondition [H] is of the form [p ~~~> n], describing the 
+    The precondition [H] is of the form [p ~~~> n], describing the
     existence of a single memory cell at location [p] with contents [n].
     The postcondition is of the form [fun v => H'], where [v] denotes
     the result and [H'] the output state.
 
     Here, the result value is unit, written [val_unit]. We employ the pure
-    fact predicate [\[v = val_unit]] to assert this equality. 
-  
+    fact predicate [\[v = val_unit]] to assert this equality.
+
     The output state is described by [p ~~~> (n+1)], describing the
     updated contents of the memory cell at location [p]. *)
 
@@ -616,11 +622,11 @@ Parameter triple_ref_with_frame : forall (l':loc) (v':val) (v:val),
 
 (** This derived specification captures the fact that the newly 
     allocated cell at address [l] is distinct from the previously
-    allocated cell at address [l']. 
+    allocated cell at address [l'].
 
     More generally, through the frame rule, we can derive that
     any piece of freshly allocated data is distinct from any 
-    piece of previously existing data. 
+    piece of previously existing data.
 
     This principle is extremely powerful. It is at the heart of
     Separation Logic. *)
@@ -641,7 +647,7 @@ Proof using.
   introv M. unfold triple in *. rename H' into H1. intros H2.
   specializes M (H1 \* H2). applys_eq M 1 2.
   { rewrite hstar_assoc. auto. }
-  { applys qprop_eq. intros v. 
+  { applys qprop_eq. intros v.
     repeat rewrite hstar_assoc. auto. }
 (* /SOLUTION *)
 Qed.
@@ -663,11 +669,11 @@ Parameter hstar_comm : forall H1 H2,
 Parameter hstar_htop_htop :
   \Top \* \Top = \Top.
 
-(* EX3! (triple_htop_post') *)
-(** Prove [triple_htop_post'], by unfolding the definition of [triple]
+(* EX3! (triple_htop_post'') *)
+(** Prove [triple_htop_post], by unfolding the definition of [triple]
     to reveal [hoare]. (However, do not unfold [hoare].) *)
 
-Lemma triple_htop_post' : forall t H Q,
+Lemma triple_htop_post'' : forall t H Q,
   triple t H (Q \*+ \Top) ->
   triple t H Q.
 Proof using.
@@ -689,8 +695,8 @@ Qed.
 (** ** Alternative definitions for heap predicates *)
 
 (** In what follows, we discuss alternative, equivalent defininitions for
-    the fundamental heap predicates. We write these equivalence using 
-    equalities of the form [H1 = H2]. We will justify later the use of 
+    the fundamental heap predicates. We write these equivalence using
+    equalities of the form [H1 = H2]. We will justify later the use of
     the equal sign for relating predicates. *)
 
 (** The empty heap predicate [\[]] is equivalent to the pure fact predicate
@@ -722,7 +728,7 @@ Proof using.
   { destruct Hh as (p&E). auto. }
 Qed.
 
-(* TODO: one of these proofs could be an exercise *)
+(* LATER: one of these proofs could be an exercise *)
 
 Definition hpure' (P:Prop) : hprop :=
   \exists (p:P), \[].
@@ -760,7 +766,7 @@ Definition htop' : hprop :=
 (* ******************************************************* *)
 (** ** Alterative definitions for SL triples *)
 
-(** We have previously defined [SL_triple] on top of [hoare],
+(** We have previously defined [triple1] on top of [hoare],
     with the help of the separating conjunction operator, as:
     [forall (H':hprop), hoare (H \* H') t (Q \*+ H')].
 
@@ -773,7 +779,7 @@ Definition htop' : hprop :=
     in such a way that [v] and [h1'] together satisfy the 
     poscondition [Q]. *)
 
-Definition SL_triple_lowlevel (t:trm) (H:hprop) (Q:val->hprop) : Prop :=
+Definition triple1_lowlevel (t:trm) (H:hprop) (Q:val->hprop) : Prop :=
   forall h1 h2,
   Fmap.disjoint h1 h2 ->
   H h1 ->
@@ -783,18 +789,18 @@ Definition SL_triple_lowlevel (t:trm) (H:hprop) (Q:val->hprop) : Prop :=
     /\ Q v h1'.
 
 (** Let us establish the equivalence between this alternative definition
-    of [SL_triple] and the original one. *)
+    of [triple1] and the original one. *)
 
-(* EX3! (SL_triple_iff_SL_triple_lowlevel) *)
-Lemma SL_triple_iff_SL_triple_lowlevel : forall t H Q,
-  SL_triple t H Q <-> SL_triple_lowlevel t H Q.
+(* EX3! (triple1_iff_triple_lowlevel) *)
+Lemma triple1_iff_triple_lowlevel : forall t H Q,
+  triple1 t H Q <-> triple1_lowlevel t H Q.
 Proof using.
 (* SOLUTION *)
-  unfold SL_triple, SL_triple_lowlevel, hoare. iff M.
+  unfold triple1, triple1_lowlevel, hoare. iff M.
   { introv D P1.
     forwards (h'&v&HR&HQ): M (=h2) (h1 \u h2). { hnf. eauto 8. }
     destruct HQ as (h1'&h2'&N0&N1&N2&N3). subst.
-    exists h1' v. eauto. }
+    exists h1' v. auto. }
   { intros H' h. introv (h1&h2&N1&N2&D&U).
     forwards (h1'&v&D'&HR&HQ): M h1 h2; auto. subst.
     exists (h1' \u h2) v. split. { eauto. } { hnf. eauto 8. } }
@@ -882,5 +888,6 @@ Proof using.
   applys M.
 (* /SOLUTION *)
 Qed.
+
 
 
